\newpage\subsection*{1551 Worksheet 7 Answers}

\SolutionsStatement

\begin{enumerate}
    
    \item \begin{enumerate}
    
    \item \begin{align*}
    	v'(t) &= \ddt 2^{3t} 
        = 2^{3t} \ln 2 \ddt (3t)  
        = 3\cdot 2^{3t} \ln 2
    \end{align*}
    Alternate solution: 
    \begin{align*}
    	v'(t) &= \ddt 2^{3t}
        = \ddt 8^t 
        = 8^t \ln 8
    \end{align*}
    
    	\item 
    	\begin{align*} 
    		y(x) &= x^{x^{x}} \\
    		\ln y&= \ln x^{x^{x}} =x^x \ln x \\
     		\frac{y'}{y} &= \ddx (x^x \ln x) \\
     		&= ( \ddx x^x ) \ln x + x^x \ddx \ln x \\
     		&= ( \ddx x^x ) \ln x + x^x \frac 1 x 
    	\end{align*}
    	Calculate the derivative of $x^x$: 
        \begin{align*}
        	\text{let } u = x^x, \text{then } \ln u &= x \ln x \\
            \frac{u'}{u} &= \ddx ( x \ln x) = \ln x + 1 \\
            u' &= u(\ln x + 1) 
            = x^x (\ln x + 1) 
        \end{align*}
        Thus $y'= x^x (\ln x + 1) \ln x + x^{x-1}$. 

        
        
        \item \begin{align*} 
        	u(x) &= \sin\left(\tan^{-1} (\ln x)\right) \\
            \ddx u 
            &= \cos\left(\tan^{-1} (\ln x)\right) \cdot 
            \ddx \left(\tan^{-1} (\ln x)\right) \\
            &= \cos\left(\tan^{-1} (\ln x)\right) \cdot 
            \frac{1}{1+ (\ln x)^2} \cdot \ddx \ln x \\    
            &= \cos\left(\tan^{-1} (\ln x)\right) \cdot 
            \frac{1}{1+ (\ln x)^2} \cdot \frac 1 x            
        \end{align*}
        
        
        
        
        \item \begin{align*} 
        	s(t) &= \log_2\left(\log_3\left(e^{t^2}\right)\right) \\
            s' 
            &= \frac{1}{\log_3\left(e^{t^2}\right) \ln 2} \cdot \ddt  \left( \log_3 e^{t^2} \right) \\
            &= \frac{1}{\log_3\left(e^{t^2}\right) \ln 2} \cdot  \frac{1}{ \log_3 e^{t^2}} \cdot \ddt e^{t^2} \\
            &= \frac{1}{\log_3\left(e^{t^2}\right) \ln 2} \cdot  \frac{1}{ \log_3 e^{t^2}} \cdot e^{t^2} \cdot 2t           
        \end{align*}
        
        
        \item \begin{align*}
        a(t) 
        &= \ln\left(\frac{(t+2)^3(t+5)^7}{\sqrt{t-5}}\right) \\
        &= 3 \ln\left(t+2 \right) + 7 \ln\left(t+5\right) - \frac 1 2 \ln \left( t-5\right) \\
        a'(t) &= \frac{3}{t+2} +\frac{7}{t+5} - \frac{1}{2(t-5)} 
        \end{align*}
    \end{enumerate}
    
    
    
    
    
    
    
    \item \begin{enumerate}
    	\item Negative. Because if the tangent line is $y=mx +b$, value of $y$ decreases as $x$ increases.
        \item Use implicit differentiation. Assume $y=y(x)$. 
        \begin{align*}
        	\ddx 2\left(x^2+y^2\right)^2&= \ddx 25\left(x^2-y^2\right) \\
        	4(x^2+y^2) \cdot (2x+ 2y y') &= 25(2x-2yy') 
        \end{align*}
        Now substitute $(3,1)$ and solve for $y'$. 
        \begin{align*}        
        	4(3^2+1^2) \cdot (2\cdot3+ 2 y') &= 25(2\cdot3-2\cdot1\cdot y')\\
        	40 (6+ 2 y') &= 25(6 - 2y')\\
             (6+ 2 y') &= \frac 5 8 (6 - 2y')\\
            \frac 13 4 y' &= - \frac 9 4 \\
            y' &= - 9 13
        \end{align*}
        Thus the equation of the tangent line is 
        \begin{align*}
        	y - 1 &= - \frac{9 }{13} (x - 3) \\
            y &= 1 - \frac{9}{ 13} (x - 3)
        \end{align*}
        The slope of the line is negative, as expected. The equation of the normal line is
        \begin{align*}
            y &= 1 + \frac{13}{ 9} (x - 3)
        \end{align*}       
    \end{enumerate}

    
\end{enumerate}    






